Compiler correctness

Compiler.lean
@@ -19,8 +19,8 @@ inductive Var (A : Typ) : (Γ : Ctx) → Type
   | succ (x : Var A Γ) : Var A (.cons Γ A')
 
 inductive Exp : (Γ : Ctx) → (A : Typ) → Type
-  | var    (x : Var A Γ)                          : Exp Γ A
-  | let    (M : Exp Γ A) (M' : Exp (Γ.cons A) A') : Exp Γ A'
+  | var (x : Var A Γ)                          : Exp Γ A
+  | let (M : Exp Γ A) (M' : Exp (Γ.cons A) A') : Exp Γ A'
 
   | absurd (M : Exp Γ .void)                                                          : Exp Γ A
   | triv                                                                              : Exp Γ .unit
@@ -36,90 +36,19 @@ inductive Exp : (Γ : Ctx) → (A : Typ) → Type
   | succ   (M : Exp Γ .nat)                                                           : Exp Γ .nat
   | iter   (M : Exp Γ .nat) (M₁ : Exp Γ A) (M₂ : Exp (Γ.cons A) A)                    : Exp Γ A
 
-  | print  (M : Exp Γ .nat) : Exp Γ .unit
-  | read                    : Exp Γ (.sum .unit .nat)
+  | print (M : Exp Γ .nat) : Exp Γ .unit
+  | read                   : Exp Γ (.sum .unit .nat)
 
-def Renaming (Γ Γ' : Ctx) : Type :=
-  ∀ {{A}}, (x : Var A Γ') → Var A Γ
+inductive Val : (M : Exp Γ A) → Type
+  | var x : Val (.var x)
 
-namespace Renaming
-
-def cons (γ : Renaming Γ Γ') (y : Var A Γ) : Renaming Γ (Γ'.cons A)
-  | _, .zero   => y
-  | _, .succ x => γ x
-
-def weaken (γ : Renaming Γ Γ') : Renaming (Γ.cons A) (Γ'.cons A) :=
-  cons (fun _ x => .succ (γ x)) .zero
-
-def apply (γ : Renaming Γ Γ') : (M : Exp Γ' A) → Exp Γ A
-  | .var x    => .var (γ x)
-  | .let M M' => .let (γ.apply M) (γ.weaken.apply M')
-
-  | .absurd M       => .absurd (γ.apply M)
-  | .triv           => .triv
-  | .inl    M       => .inl    (γ.apply M)
-  | .inr    M       => .inr    (γ.apply M)
-  | .case   M M₁ M₂ => .case   (γ.apply M) (γ.weaken.apply M₁) (γ.weaken.apply M₂)
-  | .pair   M₁ M₂   => .pair   (γ.apply M₁) (γ.apply M₂)
-  | .fst    M       => .fst    (γ.apply M)
-  | .snd    M       => .snd    (γ.apply M)
-  | .lam    M       => .lam    (γ.weaken.apply M)
-  | .ap     M M₁    => .ap     (γ.apply M) (γ.apply M₁)
-  | .zero           => .zero
-  | .succ   M       => .succ   (γ.apply M)
-  | .iter   M M₁ M₂ => .iter   (γ.apply M) (γ.apply M₁) (γ.weaken.apply M₂)
-
-  | .print  M => .print (γ.apply M)
-  | .read     => .read
-
-end Renaming
-
-def Exp.weaken : (M : Exp Γ A) → Exp (Γ.cons A') A :=
-  Renaming.apply fun _ => .succ
-
-def Subst (Γ Γ' : Ctx) : Type :=
-  ∀ {{A}}, (x : Var A Γ') → Exp Γ A
-
-namespace Subst
-
-def cons (γ : Subst Γ Γ') (M : Exp Γ A) : Subst Γ (Γ'.cons A)
-  | _, .zero   => M
-  | _, .succ x => γ x
-
-def weaken (γ : Subst Γ Γ') : Subst (Γ.cons A) (Γ'.cons A) :=
-  cons (fun _ x => (γ x).weaken) (.var .zero)
-
-def apply (γ : Subst Γ Γ') : (M : Exp Γ' A) → Exp Γ A
-  | .var x    => γ x
-  | .let M M' => .let (γ.apply M) (γ.weaken.apply M')
-
-  | .absurd M       => .absurd (γ.apply M)
-  | .triv           => .triv
-  | .inl    M       => .inl    (γ.apply M)
-  | .inr    M       => .inr    (γ.apply M)
-  | .case   M M₁ M₂ => .case   (γ.apply M) (γ.weaken.apply M₁) (γ.weaken.apply M₂)
-  | .pair   M₁ M₂   => .pair   (γ.apply M₁) (γ.apply M₂)
-  | .fst    M       => .fst    (γ.apply M)
-  | .snd    M       => .snd    (γ.apply M)
-  | .lam    M       => .lam    (γ.weaken.apply M)
-  | .ap     M M₁    => .ap     (γ.apply M) (γ.apply M₁)
-  | .zero           => .zero
-  | .succ   M       => .succ   (γ.apply M)
-  | .iter   M M₁ M₂ => .iter   (γ.apply M) (γ.apply M₁) (γ.weaken.apply M₂)
-
-  | .print  M => .print (γ.apply M)
-  | .read     => .read
-
-end Subst
-
-inductive Val : (M : Exp .nil A) → Type
-  | triv                             : Val .triv
-  | inl  (V : Val M)                 : Val (.inl M)
-  | inr  (V : Val M)                 : Val (.inr M)
-  | pair (V₁ : Val M₁) (V₂ : Val M₂) : Val (.pair M₁ M₂)
-  | lam                              : Val (.lam M)
-  | zero                             : Val .zero
-  | succ (V : Val M)                 : Val (.succ M)
+  | triv                                                 : Val .triv
+  | inl  (V : Val (A := A₁) M)                           : Val (A := .sum A₁ A₂)  (.inl M)
+  | inr  (V : Val (A := A₂) M)                           : Val (A := .sum A₁ A₂)  (.inr M)
+  | pair (V₁ : Val (A := A₁) M₁) (V₂ : Val (A := A₂) M₂) : Val (.pair M₁ M₂)
+  | lam  M                                               : Val (A := .arr A₁ A₂)  (.lam M)
+  | zero                                                 : Val .zero
+  | succ (V : Val M)                                     : Val (.succ M)
 
 instance : Subsingleton (Val M) where
   allEq V V' := by
@@ -128,18 +57,142 @@ instance : Subsingleton (Val M) where
       <;> congr
       <;> apply_assumption
 
-def Exp.subst (M : Exp (.cons .nil A') A) {M' : Exp _ A'} : (V : Val M') → Exp .nil A
-  | _ => Subst.cons (fun _ => .var) M' |>.apply M
+inductive Renaming (Γ : Ctx) : (Γ' : Ctx) → Type
+ | nil                                    : Renaming Γ .nil
+ | cons (γ : Renaming Γ Γ') (x : Var A Γ) : Renaming Γ (Γ'.cons A)
+
+@[simp]
+def Renaming.map (f : ∀ {A}, (x : Var A Γ) → Var A Γ'') : (γ : Renaming Γ Γ') → Renaming Γ'' Γ'
+  | nil      => nil
+  | cons γ x => cons (γ.map @f) (f x)
+
+@[simp]
+def Renaming.weaken (γ : Renaming Γ Γ') : Renaming (Γ.cons A) (Γ'.cons A) :=
+  cons (γ.map .succ) .zero
+
+def Renaming.id : ∀ {Γ}, Renaming Γ Γ
+  | .nil     => nil
+  | .cons .. => cons (map .succ id) .zero
+
+@[simp]
+theorem Renaming.map_map : map f (map g γ) = γ.map (f <| g ·) :=
+  by induction γ <;> simp [*]
+
+@[simp]
+def Var.rename : (γ : Renaming Γ Γ') → (x : Var A Γ') → Var A Γ
+  | .cons _ x, zero   => x
+  | .cons γ _, succ x => x.rename γ
+
+@[simp]
+theorem Var.rename_map : rename (.map f γ) x = f (x.rename γ) :=
+  by induction x <;> cases γ <;> apply_assumption
+
+@[simp]
+theorem Var.rename_id : rename .id x = x :=
+  by induction x <;> simp [*]
+
+@[simp]
+theorem Renaming.map_rename {γ : Renaming Γ Γ'} : map (f <| ·.rename γ) .id = map f γ :=
+  by induction γ <;> simp [*]
+
+def Exp.rename (γ : Renaming Γ Γ') : (M : Exp Γ' A) → Exp Γ A
+  | .var x    => .var (x.rename γ)
+  | .let M M' => .let (M.rename γ) (M'.rename γ.weaken)
+
+  | absurd M       => absurd (M.rename γ)
+  | triv           => triv
+  | inl    M       => inl    (M.rename γ)
+  | inr    M       => inr    (M.rename γ)
+  | case   M M₁ M₂ => case   (M.rename γ) (M₁.rename γ.weaken) (M₂.rename γ.weaken)
+  | pair   M₁ M₂   => pair   (M₁.rename γ) (M₂.rename γ)
+  | fst    M       => fst    (M.rename γ)
+  | snd    M       => snd    (M.rename γ)
+  | lam    M       => lam    (M.rename γ.weaken)
+  | ap     M M₁    => ap     (M.rename γ) (M₁.rename γ)
+  | zero           => zero
+  | succ   M       => succ   (M.rename γ)
+  | iter   M M₁ M₂ => iter   (M.rename γ) (M₁.rename γ) (M₂.rename γ.weaken)
+
+  | print M => print (M.rename γ)
+  | read    => read
+
+def Val.rename (γ : Renaming Γ Γ') : (V : Val (A := A) M) → Val (M.rename γ)
+  | var x => var _
+
+  | triv       => triv
+  | inl  V     => inl  (V.rename γ)
+  | inr  V     => inr  (V.rename γ)
+  | pair V₁ V₂ => pair (V₁.rename γ) (V₂.rename γ)
+  | lam  M     => lam  _
+  | zero       => zero
+  | succ V     => succ (V.rename γ)
+
+def Exp.weaken : (M : Exp Γ A) → Exp (Γ.cons A') A :=
+  rename (.map .succ .id)
+
+def Val.weaken : (V : @Val Γ A M) → Val (M.weaken (A' := A')) :=
+  rename (.map .succ .id)
+
+inductive Subst (Γ : Ctx) : (Γ' : Ctx) → Type
+ | nil                                    : Subst Γ .nil
+ | cons (γ : Subst Γ Γ') (V : @Val Γ A M) : Subst Γ (Γ'.cons A)
+
+def Subst.map {f : ∀ {A}, (M : Exp Γ A) → Exp Γ'' A} (g : ∀ {A M}, (V : Val M) → Val (@f A M)) : (γ : Subst Γ Γ') → Subst Γ'' Γ'
+  | nil      => nil
+  | cons γ M => cons (γ.map (f := @f) @g) (g M)
+
+def Subst.weaken (γ : Subst Γ Γ') : Subst (Γ.cons A) (Γ'.cons A) :=
+  cons (γ.map .weaken) (.var .zero)
+
+@[simp]
+def Subst.ofRenaming {f : ∀ {A}, (x : Var A Γ) → Exp Γ'' A} (g : ∀ {A}, (x : Var A Γ) → Val (f x)) : (γ : Renaming Γ Γ') → Subst Γ'' Γ'
+  | .nil      => nil
+  | .cons γ x => cons (ofRenaming (f := @f) @g γ) (g x)
+
+@[simp]
+theorem Subst.ofRenaming_map : ofRenaming f (γ.map g) = ofRenaming (f <| g ·) γ :=
+  by induction γ <;> simp [*]
+
+@[simp]
+def Var.subst : (γ : Subst Γ Γ') → (x : Var A Γ') → Exp Γ A
+  | .cons (M := M) .., zero   => M
+  | .cons γ _,         succ x => x.subst γ
+
+@[simp]
+def Exp.subst (γ : Subst Γ Γ') : (M : Exp Γ' A) → Exp Γ A
+  | .var x    => x.subst γ
+  | .let M M' => .let (M.subst γ) (M'.subst γ.weaken)
+
+  | absurd M       => absurd (M.subst γ)
+  | triv           => triv
+  | inl    M       => inl    (M.subst γ)
+  | inr    M       => inr    (M.subst γ)
+  | case   M M₁ M₂ => case   (M.subst γ) (M₁.subst γ.weaken) (M₂.subst γ.weaken)
+  | pair   M₁ M₂   => pair   (M₁.subst γ) (M₂.subst γ)
+  | fst    M       => fst    (M.subst γ)
+  | snd    M       => snd    (M.subst γ)
+  | lam    M       => lam    (M.subst γ.weaken)
+  | ap     M M₁    => ap     (M.subst γ) (M₁.subst γ)
+  | zero           => zero
+  | succ   M       => succ   (M.subst γ)
+  | iter   M M₁ M₂ => iter   (M.subst γ) (M₁.subst γ) (M₂.subst γ.weaken)
+
+  | print M => print (M.subst γ)
+  | read    => read
+
+def Exp.sub (M : Exp (Γ.cons A') A) {M' : Exp Γ A'} (V : Val M') : Exp Γ A :=
+  subst (.cons (.ofRenaming .var .id) V) M
 
 def Exp.ofNat : (n : Nat) → Exp Γ .nat
   | .zero   => zero
   | .succ n => succ (ofNat n)
 
-def Val.ofNat : (n : Nat) → Val (.ofNat n)
+def Val.ofNat : (n : Nat) → Val (.ofNat (Γ := Γ) n)
   | .zero   => zero
   | .succ n => succ (ofNat n)
 
-def Val.toNat {M : Exp _ .nat} : (V : Val M) → Nat
+@[simp]
+def Val.toNat : (V : @Val .nil .nat M) → Nat
   | zero   => .zero
   | succ V => .succ V.toNat
 
@@ -163,12 +216,12 @@ inductive Steps : (S S' : State A) → Type
   | ap₁                 (s  : Steps (I, M,  O) (I', M',  O')) : Steps (I, .ap   M  M₁, O) (I', .ap   M'  M₁,  O')
   | ap₂   (V  : Val M)  (s₁ : Steps (I, M₁, O) (I', M₁', O')) : Steps (I, .ap   M  M₁, O) (I', .ap   M   M₁', O')
 
-  | let'      (V : Val M)                 : Steps (I, .let M M',             O) (I, M'.subst V,              O)
-  | case_inl  (V : Val M)                 : Steps (I, .case (.inl M) M₁ M₂,  O) (I, M₁.subst V,              O)
-  | case_inr  (V : Val M)                 : Steps (I, .case (.inr M) M₁ M₂,  O) (I, M₂.subst V,              O)
+  | let'      (V : Val M)                 : Steps (I, .let M M',             O) (I, M'.sub V,                O)
+  | case_inl  (V : Val M)                 : Steps (I, .case (.inl M) M₁ M₂,  O) (I, M₁.sub V,                O)
+  | case_inr  (V : Val M)                 : Steps (I, .case (.inr M) M₁ M₂,  O) (I, M₂.sub V,                O)
   | fst_pair  (V₁ : Val M₁) (V₂ : Val M₂) : Steps (I, .fst (.pair M₁ M₂),    O) (I, M₁,                      O)
   | snd_pair  (V₁ : Val M₁) (V₂ : Val M₂) : Steps (I, .snd (.pair M₁ M₂),    O) (I, M₂,                      O)
-  | ap_lam    (V₁ : Val M₁)               : Steps (I, .ap (.lam M) M₁,       O) (I, M.subst V₁,              O)
+  | ap_lam    (V₁ : Val M₁)               : Steps (I, .ap (.lam M) M₁,       O) (I, M.sub V₁,                O)
   | iter_zero                             : Steps (I, .iter .zero M₁ M₂,     O) (I, M₁,                      O)
   | iter_succ (V : Val M)                 : Steps (I, .iter (.succ M) M₁ M₂, O) (I, .let (.iter M M₁ M₂) M₂, O)
 
@@ -186,6 +239,10 @@ theorem Final.not_steps (V : Final S) (s : Steps S S') : False := by
     <;> cases s
     <;> solve_by_elim
 
+inductive Progress (S : State A)
+  | final (V : Final S)
+  | steps (s : Steps S S')
+
 instance : Subsingleton (Σ S', Steps S S') where
   allEq := by
     intro ⟨S', s⟩ ⟨S'', s'⟩
@@ -199,85 +256,54 @@ instance : Subsingleton (Σ S', Steps S S') where
       <;> congr
       <;> apply Subsingleton.allEq
 
-def progress : (S : State A) → Final S ⊕ Σ S', Steps S S'
+instance : Subsingleton (Progress S) where
+  allEq
+    | .final V₁, .final V₂ => match Subsingleton.allEq (α := Val _) V₁ V₂ with | rfl => rfl
+    | .final V₁, .steps s₂ => nomatch V₁.not_steps s₂
+    | .steps s₁, .final V₂ => nomatch V₂.not_steps s₁
+    | .steps s₁, .steps s₂ => match Subsingleton.allEq (α := Σ _, _) ⟨_, s₁⟩ ⟨_, s₂⟩ with | rfl => rfl
+
+def Progress.then (f : Exp _ A → Exp _ A')
+  (steps : ∀ {I₁' M₁' O₁'}, Steps (I₁, M₁, O₁) (I₁', M₁', O₁') → Steps (I₁, f M₁, O₁) (I₁', f M₁', O₁'))
+  (final : Final (I₁, M₁, O₁) → Progress (I₁, f M₁, O₁))
+: Progress (I₁, M₁, O₁) → Progress (I₁, f M₁, O₁)
+  | .steps s => .steps (steps s)
+  | .final V => final V
+
+def progress : (S : State A) → Progress S
   | (_, M, _) => progress M
-  where progress {A I O} : (M : Exp _ A) → Final (I, M, O) ⊕ Σ S', Steps (I, M, O) S'
-    | .let M _ => match progress M with
-                  | .inl V      => .inr ⟨_, .let' V⟩
-                  | .inr ⟨_, s⟩ => .inr ⟨_, .let s⟩
+  where progress {A I O} : (M : Exp _ A) → Progress (I, M, O)
+    | .let M _ => progress M |>.then (.let · _) .let fun V => .steps <| .let' V
 
-    | .absurd M     => match progress M with
-                       | .inr ⟨_, s⟩ => .inr ⟨_, .absurd s⟩
-    | .triv         => .inl .triv
-    | .inl    M     => match progress M with
-                       | .inl V      => .inl (.inl V)
-                       | .inr ⟨_, s⟩ => .inr ⟨_, .inl s⟩
-    | .inr    M     => match progress M with
-                       | .inl V      => .inl (.inr V)
-                       | .inr ⟨_, s⟩ => .inr ⟨_, .inr s⟩
-    | .case   M ..  => match progress M with
-                       | .inl (.inl V) => .inr ⟨_, .case_inl V⟩
-                       | .inl (.inr V) => .inr ⟨_, .case_inr V⟩
-                       | .inr ⟨_, s⟩   => .inr ⟨_, .case s⟩
-    | .pair   M₁ M₂ => match progress M₁, progress M₂ with
-                       | .inl V₁,      .inl V₂      => .inl (.pair V₁ V₂)
-                       | .inl V₁,      .inr ⟨_, s₂⟩ => .inr ⟨_, .pair₂ V₁ s₂⟩
-                       | .inr ⟨_, s₁⟩, _            => .inr ⟨_, .pair₁ s₁⟩
-    | .fst    M     => match progress M with
-                       | .inl (.pair V₁ V₂) => .inr ⟨_, .fst_pair V₁ V₂⟩
-                       | .inr ⟨_, s⟩        => .inr ⟨_, .fst s⟩
-    | .snd    M     => match progress M with
-                       | .inl (.pair V₁ V₂) => .inr ⟨_, .snd_pair V₁ V₂⟩
-                       | .inr ⟨_, s⟩        => .inr ⟨_, .snd s⟩
-    | .lam    _     => .inl .lam
-    | .ap     M M₁  => match progress M, progress M₁ with
-                       | .inl .lam,   .inl V₁      => .inr ⟨_, .ap_lam V₁⟩
-                       | .inl V,      .inr ⟨_, s₁⟩ => .inr ⟨_, .ap₂ V s₁⟩
-                       | .inr ⟨_, s⟩, _            => .inr ⟨_, .ap₁ s⟩
-    | .zero         => .inl .zero
-    | .succ   M     => match progress M with
-                       | .inl V      => .inl (.succ V)
-                       | .inr ⟨_, s⟩ => .inr ⟨_, .succ s⟩
-    | .iter   M ..  => match progress M with
-                       | .inl .zero     => .inr ⟨_, .iter_zero⟩
-                       | .inl (.succ V) => .inr ⟨_, .iter_succ V⟩
-                       | .inr ⟨_, s⟩    => .inr ⟨_, .iter s⟩
+    | .absurd M     => progress M |>.then .absurd .absurd nofun
+    | .triv         => .final .triv
+    | .inl    M     => progress M |>.then .inl .inl fun V => .final <| .inl V
+    | .inr    M     => progress M |>.then .inr .inr fun V => .final <| .inr V
+    | .case   M ..  => progress M |>.then (.case · ..) .case fun | .inl V => .steps <| .case_inl V | .inr V => .steps <| .case_inr V
+    | .pair   M₁ M₂ => progress M₁ |>.then (.pair · _) .pair₁ fun V₁ => progress M₂ |>.then (.pair _) (.pair₂ V₁) fun V₂ => .final <| .pair V₁ V₂
+    | .fst    M     => progress M |>.then .fst .fst fun | .pair V₁ V₂ => .steps <| .fst_pair V₁ V₂
+    | .snd    M     => progress M |>.then .snd .snd fun | .pair V₁ V₂ => .steps <| .snd_pair V₁ V₂
+    | .lam    M     => .final <| .lam M
+    | .ap     M M₁  => progress M |>.then (.ap · _) .ap₁ fun | V@(.lam _) => progress M₁ |>.then (.ap _) (.ap₂ V) fun V₁ => .steps <| .ap_lam V₁
+    | .zero         => .final .zero
+    | .succ   M     => progress M |>.then .succ .succ fun V => .final <| .succ V
+    | .iter   M ..  => progress M |>.then (.iter · ..) .iter fun | .zero => .steps .iter_zero | .succ V => .steps <| .iter_succ V
 
-    | .print M => match progress M with
-                  | .inl V      => .inr ⟨_, .print' V⟩
-                  | .inr ⟨_, s⟩ => .inr ⟨_, .print s⟩
+    | .print M => progress M |>.then .print .print fun V => .steps <| .print' V
     | .read    => match I with
-                  | []     => .inr ⟨_, .read₁⟩
-                  | n :: I => .inr ⟨_, .read₂⟩
-
-instance : Subsingleton (Final S ⊕ Σ S', Steps S S') where
-  allEq S₁ S₂ := by
-    match S₁ with
-    | .inl V₁ =>
-      match S₂ with
-      | .inl V₂ =>
-        cases Subsingleton.elim (α := Val _) V₁ V₂
-        rfl
-      | .inr ⟨S₂, s₂⟩ =>
-        nomatch V₁.not_steps s₂
-    | .inr ⟨S₁, s₁⟩ =>
-      match S₂ with
-      | .inl V₂ =>
-        nomatch V₂.not_steps s₁
-      | .inr ⟨S₂, s₂⟩ =>
-        cases Subsingleton.elim (α := Σ _, _) ⟨S₁, s₁⟩ ⟨S₂, s₂⟩
-        rfl
+                  | []     => .steps .read₁
+                  | _ :: _ => .steps .read₂
 
 end CBV
 
 namespace Modal
 
-export CBV (Typ Ctx Var)
+export CBV (Typ Ctx Var Renaming)
 
 mutual
 
 inductive Val : (Γ : Ctx) → (A : Typ) → Type
-  | var  (x : Var A Γ)                   : Val Γ A
+  | var (x : Var A Γ) : Val Γ A
 
   | triv                                 : Val Γ .unit
   | inl  (V : Val Γ A₁)                  : Val Γ (.sum A₁ A₂)
@@ -288,8 +314,8 @@ inductive Val : (Γ : Ctx) → (A : Typ) → Type
   | succ (V : Val Γ .nat)                : Val Γ .nat
 
 inductive Exp : (Γ : Ctx) → (A : Typ) → Type
-  | ret    (V : Val Γ A)                                                              : Exp Γ A
-  | let    (M : Exp Γ A) (M' : Exp (Γ.cons A) A')                                     : Exp Γ A'
+  | ret (V : Val Γ A)                          : Exp Γ A
+  | let (M : Exp Γ A) (M' : Exp (Γ.cons A) A') : Exp Γ A'
 
   | absurd (V : Val Γ .void)                                                          : Exp Γ A
   | case   (V : Val Γ (.sum A₁ A₂)) (M₁ : Exp (Γ.cons A₁) A) (M₂ : Exp (Γ.cons A₂) A) : Exp Γ A
@@ -298,117 +324,211 @@ inductive Exp : (Γ : Ctx) → (A : Typ) → Type
   | ap     (V : Val Γ (.arr A₁ A₂)) (V₁ : Val Γ A₁)                                   : Exp Γ A₂
   | iter   (V : Val Γ .nat) (M₁ : Exp Γ A) (M₂ : Exp (Γ.cons A) A)                    : Exp Γ A
 
-  | print  (V : Val Γ .nat)                                                           : Exp Γ .unit
-  | read                                                                              : Exp Γ (.sum .unit .nat)
+  | print (V : Val Γ .nat) : Exp Γ .unit
+  | read                   : Exp Γ (.sum .unit .nat)
 
 end
 
-def Renaming (Γ Γ' : Ctx) : Type :=
-  ∀ {{A}}, (x : Var A Γ') → Var A Γ
-
-namespace Renaming
-
-def cons (γ : Renaming Γ Γ') (y : Var A Γ) : Renaming Γ (Γ'.cons A)
-  | _, .zero   => y
-  | _, .succ x => γ x
-
-def weaken (γ : Renaming Γ Γ') : Renaming (Γ.cons A) (Γ'.cons A) :=
-  cons (fun _ x => .succ (γ x)) .zero
-
+set_option linter.unusedVariables false in
 @[structural]
 mutual
 
-def applyV (γ : Renaming Γ Γ') : (V : Val Γ' A) → Val Γ A
-  | .var  x     => .var  (γ x)
-  | .triv       => .triv
-  | .inl  V     => .inl  (γ.applyV V)
-  | .inr  V     => .inr  (γ.applyV V)
-  | .pair V₁ V₂ => .pair (γ.applyV V₁) (γ.applyV V₂)
-  | .lam  M     => .lam  (γ.weaken.applyE M)
-  | .zero       => .zero
-  | .succ V     => .succ (γ.applyV V)
+@[simp]
+def Val.rename (γ : Renaming Γ Γ') : (V : Val Γ' A) → Val Γ A
+  | .var x => .var (x.rename γ)
 
-def applyE (γ : Renaming Γ Γ') : (M : Exp Γ' A) → Exp Γ A
-  | .ret    V       => .ret    (γ.applyV V)
-  | .let    M M'    => .let    (γ.applyE M) (γ.weaken.applyE M')
-  | .absurd V       => .absurd (γ.applyV V)
-  | .case   V M₁ M₂ => .case   (γ.applyV V) (γ.weaken.applyE M₁) (γ.weaken.applyE M₂)
-  | .fst    V       => .fst    (γ.applyV V)
-  | .snd    V       => .snd    (γ.applyV V)
-  | .ap     V V₁    => .ap     (γ.applyV V) (γ.applyV V₁)
-  | .iter   V M₁ M₂ => .iter   (γ.applyV V) (γ.applyE M₁) (γ.weaken.applyE M₂)
-  | .print  V       => .print  (γ.applyV V)
-  | .read           => .read
+  | .triv       => .triv
+  | .inl  V     => .inl  (V.rename γ)
+  | .inr  V     => .inr  (V.rename γ)
+  | .pair V₁ V₂ => .pair (V₁.rename γ) (V₂.rename γ)
+  | .lam  M     => .lam  (M.rename γ.weaken)
+  | .zero       => .zero
+  | .succ V     => .succ (V.rename γ)
+
+@[simp]
+def Exp.rename (γ : Renaming Γ Γ') : (M : Exp Γ' A) → Exp Γ A
+  | .ret V    => .ret (V.rename γ)
+  | .let M M' => .let (M.rename γ) (M'.rename γ.weaken)
+
+  | .absurd V       => .absurd (V.rename γ)
+  | .case   V M₁ M₂ => .case   (V.rename γ) (M₁.rename γ.weaken) (M₂.rename γ.weaken)
+  | .fst    V       => .fst    (V.rename γ)
+  | .snd    V       => .snd    (V.rename γ)
+  | .ap     V V₁    => .ap     (V.rename γ) (V₁.rename γ)
+  | .iter   V M₁ M₂ => .iter   (V.rename γ) (M₁.rename γ) (M₂.rename γ.weaken)
+
+  | .print V => .print (V.rename γ)
+  | .read    => .read
 
 end
 
-end Renaming
+@[simp]
+theorem Val.rename_rename {γ : Renaming Γ Γ'} {γ' : Renaming Γ' Γ''} : (rename γ' V).rename γ = V.rename (γ'.map (·.rename γ)) := by
+  induction V
+    using Val.rec (motive_2 := fun Γ'' A M => ∀ {Γ Γ'}, {γ : Renaming Γ Γ'} → {γ' : Renaming Γ' Γ''} → (M.rename γ').rename γ = M.rename (γ'.map (·.rename γ)))
+    generalizing Γ Γ'
+    <;> simp [*]
+
+@[simp]
+theorem Exp.rename_rename {γ : Renaming Γ Γ'} {γ' : Renaming Γ' Γ''} : (rename γ' M).rename γ = M.rename (γ'.map (·.rename γ)) := by
+  induction M
+    using Exp.rec (motive_1 := fun Γ'' A V => ∀ {Γ Γ'}, {γ : Renaming Γ Γ'} → {γ' : Renaming Γ' Γ''} → (V.rename γ').rename γ = V.rename (γ'.map (·.rename γ)))
+    generalizing Γ Γ'
+    <;> simp [*]
 
 @[simp]
 def Val.weaken : (V : Val Γ A) → Val (Γ.cons A') A :=
-  Renaming.applyV fun _ => .succ
+  rename (.map .succ .id)
 
 @[simp]
 def Exp.weaken : (M : Exp Γ A) → Exp (Γ.cons A') A :=
-  Renaming.applyE fun _ => .succ
+  rename (.map .succ .id)
 
 @[simp]
 def Exp.weaken₁ : (M : Exp (.cons Γ A') A) → Exp ((Γ.cons A'').cons A') A :=
-  Renaming.cons (fun _ x => x.succ.succ) .zero |>.applyE
+  rename (.cons (.map (·.succ.succ) .id) .zero)
 
-def Subst (Γ Γ' : Ctx) : Type :=
-  ∀ {{A}}, (x : Var A Γ') → Val Γ A
-
-namespace Subst
-
-@[simp]
-def cons (γ : Subst Γ Γ') (V : Val Γ A) : Subst Γ (Γ'.cons A)
-  | _, .zero   => V
-  | _, .succ x => γ x
+inductive Subst (Γ : Ctx) : (Γ' : Ctx) → Type
+ | nil                                 : Subst Γ .nil
+ | cons (γ : Subst Γ Γ') (M : Val Γ A) : Subst Γ (Γ'.cons A)
 
 @[simp]
-def weaken (γ : Subst Γ Γ') : Subst (Γ.cons A) (Γ'.cons A) :=
-  cons (fun _ x => (γ x).weaken) (.var .zero)
+def Subst.map (f : ∀ {A}, (M : Val Γ A) → Val Γ'' A) : (γ : Subst Γ Γ') → Subst Γ'' Γ'
+  | nil      => nil
+  | cons γ M => cons (γ.map @f) (f M)
 
+@[simp]
+def Subst.weaken (γ : Subst Γ Γ') : Subst (Γ.cons A) (Γ'.cons A) :=
+  cons (γ.map .weaken) (.var .zero)
+
+@[simp]
+def Subst.ofRenaming (f : ∀ {A}, Var A Γ → Val Γ'' A) : (γ : Renaming Γ Γ') → Subst Γ'' Γ'
+  | .nil      => nil
+  | .cons γ x => cons (ofRenaming @f γ) (f x)
+
+@[simp]
+theorem Subst.ofRenaming_map : ofRenaming f (γ.map g) = ofRenaming (f <| g ·) γ :=
+  by induction γ <;> simp [*]
+
+@[simp]
+theorem Subst.map_ofRenaming : (ofRenaming g γ).map f = ofRenaming (f <| g ·) γ :=
+  by induction γ <;> simp [*]
+
+@[simp]
+theorem Subst.map_map : map f (map g γ) = γ.map (f <| g ·) :=
+  by induction γ <;> simp [*]
+
+@[simp]
+def Var.subst : (γ : Subst Γ Γ') → (x : Var A Γ') → Val Γ A
+  | .cons _ M, .zero   => M
+  | .cons γ _, .succ x => subst γ x
+
+@[simp]
+theorem Var.subst_ofRenaming : subst (.ofRenaming f γ) x = f (x.rename γ) :=
+  by induction x <;> cases γ <;> apply_assumption
+
+@[simp]
+theorem Var.subst_map : subst (.map f γ) x = f (subst γ x) :=
+  by induction x <;> cases γ <;> apply_assumption
+
+@[simp]
+theorem Subst.ofRenaming_subst {γ : Subst Γ Γ'} : ofRenaming (f <| Var.subst γ ·) .id = .map f γ :=
+  by induction γ <;> simp [*]
+
+set_option linter.unusedVariables false in
 @[structural]
 mutual
 
 @[simp]
-def applyV (γ : Subst Γ Γ') : (V : Val Γ' A) → Val Γ A
-  | .var  x     => γ x
+def Val.subst (γ : Subst Γ Γ') : (V : Val Γ' A) → Val Γ A
+  | .var x => Var.subst γ x
+
   | .triv       => .triv
-  | .inl  V     => .inl  (γ.applyV V)
-  | .inr  V     => .inr  (γ.applyV V)
-  | .pair V₁ V₂ => .pair (γ.applyV V₁) (γ.applyV V₂)
-  | .lam  M     => .lam  (γ.weaken.applyE M)
+  | .inl  V     => .inl  (V.subst γ)
+  | .inr  V     => .inr  (V.subst γ)
+  | .pair V₁ V₂ => .pair (V₁.subst γ) (V₂.subst γ)
+  | .lam  M     => .lam  (M.subst γ.weaken)
   | .zero       => .zero
-  | .succ V     => .succ (γ.applyV V)
+  | .succ V     => .succ (V.subst γ)
 
 @[simp]
-def applyE (γ : Subst Γ Γ') : (M : Exp Γ' A) → Exp Γ A
-  | .ret    V       => .ret    (γ.applyV V)
-  | .let    M M'    => .let    (γ.applyE M) (γ.weaken.applyE M')
-  | .absurd V       => .absurd (γ.applyV V)
-  | .case   V M₁ M₂ => .case   (γ.applyV V) (γ.weaken.applyE M₁) (γ.weaken.applyE M₂)
-  | .fst    V       => .fst    (γ.applyV V)
-  | .snd    V       => .snd    (γ.applyV V)
-  | .ap     V V₁    => .ap     (γ.applyV V) (γ.applyV V₁)
-  | .iter   V M₁ M₂ => .iter   (γ.applyV V) (γ.applyE M₁) (γ.weaken.applyE M₂)
-  | .print  V       => .print  (γ.applyV V)
-  | .read           => .read
+def Exp.subst (γ : Subst Γ Γ') : (M : Exp Γ' A) → Exp Γ A
+  | .ret V    => .ret (V.subst γ)
+  | .let M M' => .let (M.subst γ) (M'.subst γ.weaken)
+
+  | .absurd V       => .absurd (V.subst γ)
+  | .case   V M₁ M₂ => .case   (V.subst γ) (M₁.subst γ.weaken) (M₂.subst γ.weaken)
+  | .fst    V       => .fst    (V.subst γ)
+  | .snd    V       => .snd    (V.subst γ)
+  | .ap     V V₁    => .ap     (V.subst γ) (V₁.subst γ)
+  | .iter   V M₁ M₂ => .iter   (V.subst γ) (M₁.subst γ) (M₂.subst γ.weaken)
+
+  | .print V => .print (V.subst γ)
+  | .read    => .read
 
 end
 
-end Subst
+@[simp]
+theorem Val.subst_id : subst (.ofRenaming .var .id) V = V := by
+  induction V
+    using Val.rec (motive_2 := fun Γ A M => M.subst (.ofRenaming .var .id) = M)
+    <;> simp_all
 
 @[simp]
-def Exp.subst (M : Exp (.cons Γ A') A) (V : Val Γ A') : Exp Γ A :=
-  Subst.cons (fun _ => .var) V |>.applyE M
+theorem Exp.subst_id : subst (.ofRenaming .var .id) M = M := by
+  induction M
+    using Exp.rec (motive_1 := fun Γ A V => V.subst (.ofRenaming .var .id) = V)
+    <;> simp_all
+
+@[simp]
+theorem Val.subst_nil : subst .nil V = V :=
+  subst_id
+
+@[simp]
+theorem Exp.subst_nil : subst .nil M = M :=
+  subst_id
+
+@[simp]
+theorem Exp.subst_cons_nil_zero : subst (.cons .nil (.var .zero)) M = M :=
+  subst_id
+
+@[simp]
+theorem Val.subst_rename {γ : Subst Γ Γ'} {γ' : Renaming Γ' Γ''} : (rename γ' V).subst γ = V.subst (.ofRenaming (Var.subst γ) γ') := by
+  induction V
+    using Val.rec (motive_2 := fun Γ'' A M => ∀ {Γ Γ'}, {γ : Subst Γ Γ'} → {γ' : Renaming Γ' Γ''} → (M.rename γ').subst γ = M.subst (.ofRenaming (Var.subst γ) γ'))
+    generalizing Γ Γ'
+    <;> simp [*]
+
+@[simp]
+theorem Exp.subst_rename {γ : Subst Γ Γ'} {γ' : Renaming Γ' Γ''} : (rename γ' M).subst γ = M.subst (.ofRenaming (Var.subst γ) γ') := by
+  induction M
+    using Exp.rec (motive_1 := fun Γ'' A V => ∀ {Γ Γ'}, {γ : Subst Γ Γ'} → {γ' : Renaming Γ' Γ''} → (V.rename γ').subst γ = V.subst (.ofRenaming (Var.subst γ) γ'))
+    generalizing Γ Γ'
+    <;> simp [*]
+
+@[simp]
+theorem Val.rename_subst {γ : Renaming Γ Γ'} {γ' : Subst Γ' Γ''} : (subst γ' V).rename γ = V.subst (.map (.rename γ) γ') := by
+  induction V
+    using Val.rec (motive_2 := fun Γ'' A M => ∀ {Γ Γ'}, {γ : Renaming Γ Γ'} → {γ' : Subst Γ' Γ''} → (M.subst γ').rename γ = M.subst (.map (.rename γ) γ'))
+    generalizing Γ Γ'
+    <;> simp [*]
+
+@[simp]
+theorem Exp.rename_subst {γ : Renaming Γ Γ'} {γ' : Subst Γ' Γ''} : (subst γ' M).rename γ = M.subst (.map (.rename γ) γ') := by
+  induction M
+    using Exp.rec (motive_1 := fun Γ'' A V => ∀ {Γ Γ'}, {γ : Renaming Γ Γ'} → {γ' : Subst Γ' Γ''} → (V.subst γ').rename γ = V.subst (.map (.rename γ) γ'))
+    generalizing Γ Γ'
+    <;> simp [*]
+
+@[simp]
+def Exp.sub (M : Exp (.cons Γ A') A) (V : Val Γ A') : Exp Γ A :=
+  subst (.cons (.ofRenaming .var .id) V) M
 
 def Val.ofNat : (n : Nat) → Val Γ .nat
   | .zero   => zero
   | .succ n => succ (ofNat n)
 
+@[simp]
 def Val.toNat : (V : Val .nil .nat) → Nat
   | zero   => .zero
   | succ V => .succ V.toNat
@@ -418,13 +538,13 @@ def State (A : Typ) : Type :=
 
 inductive Steps : (S S' : State A) → Type
   | let₁ (s : Steps (I, M, O) (I', M', O')) : Steps (I, .let M M'',      O) (I', .let M' M'', O')
-  | let₂                                    : Steps (I, .let (.ret V) M, O) (I, M.subst V, O)
+  | let₂                                    : Steps (I, .let (.ret V) M, O) (I, M.sub V,      O)
 
-  | case_inl  : Steps (I, .case (.inl V) M₁ M₂,  O) (I, M₁.subst V,              O)
-  | case_inr  : Steps (I, .case (.inr V) M₁ M₂,  O) (I, M₂.subst V,              O)
+  | case_inl  : Steps (I, .case (.inl V) M₁ M₂,  O) (I, M₁.sub V,                O)
+  | case_inr  : Steps (I, .case (.inr V) M₁ M₂,  O) (I, M₂.sub V,                O)
   | fst_pair  : Steps (I, .fst (.pair V₁ V₂),    O) (I, .ret V₁,                 O)
   | snd_pair  : Steps (I, .snd (.pair V₁ V₂),    O) (I, .ret V₂,                 O)
-  | ap_lam    : Steps (I, .ap (.lam M) V₁,       O) (I, M.subst V₁,              O)
+  | ap_lam    : Steps (I, .ap (.lam M) V₁,       O) (I, M.sub V₁,                O)
   | iter_zero : Steps (I, .iter .zero M₁ M₂,     O) (I, M₁,                      O)
   | iter_succ : Steps (I, .iter (.succ V) M₁ M₂, O) (I, .let (.iter V M₁ M₂) M₂, O)
 
@@ -436,11 +556,14 @@ inductive Final : (S : State A) → Type
   | ret : Final (I, .ret V, O)
 
 instance : Subsingleton (Final S) where
-  allEq := by
-    intro .ret .ret
-    rfl
+  allEq
+    | .ret, .ret => rfl
 
 theorem Final.not_steps : (V : Final S) → (s : Steps S S') → False := nofun
+
+inductive Progress (S : State A)
+  | final (r : Final S)
+  | steps (s : Steps S S')
 
 instance : Subsingleton (Σ S', Steps S S') where
   allEq := by
@@ -452,44 +575,33 @@ instance : Subsingleton (Σ S', Steps S S') where
       <;> (try rfl)
       <;> nomatch Final.not_steps .ret ‹_›
 
-def progress : (S : State A) → Final S ⊕ Σ S', Steps S S'
-  | (I, M, O) => progress I O M
-  where progress {A} I O : (M : Exp _ A) → Final (I, M, O) ⊕ Σ S', Steps (I, M, O) S'
-    | .ret V    => .inl .ret
-    | .let M M' => match progress I O M with
-                   | .inl .ret   => .inr ⟨_, .let₂⟩
-                   | .inr ⟨_, s⟩ => .inr ⟨_, .let₁ s⟩
+instance : Subsingleton (Progress S) where
+  allEq
+    | .final r₁, .final r₂ => match Subsingleton.allEq r₁ r₂ with | rfl => rfl
+    | .final r₁, .steps s₂ => nomatch r₁.not_steps s₂
+    | .steps s₁, .final r₂ => nomatch r₂.not_steps s₁
+    | .steps s₁, .steps s₂ => match Subsingleton.allEq (α := Σ _, _) ⟨_, s₁⟩ ⟨_, s₂⟩ with | rfl => rfl
 
-    | .case (.inl _) ..  => .inr ⟨_, .case_inl⟩
-    | .case (.inr _) ..  => .inr ⟨_, .case_inr⟩
-    | .fst  (.pair ..)   => .inr ⟨_, .fst_pair⟩
-    | .snd  (.pair ..)   => .inr ⟨_, .snd_pair⟩
-    | .ap   (.lam _) _   => .inr ⟨_, .ap_lam⟩
-    | .iter .zero ..     => .inr ⟨_, .iter_zero⟩
-    | .iter (.succ _) .. => .inr ⟨_, .iter_succ⟩
+def progress : (S : State A) → Progress S
+  | (_, M, _) => progress M
+  where progress {A I O} : (M : Exp _ A) → Progress (I, M, O)
+    | .ret V    => .final .ret
+    | .let M M' => match M, progress M with
+                   | _, .steps s    => .steps (.let₁ s)
+                   | _, .final .ret => .steps .let₂
 
-    | .print _ => .inr ⟨_, .print⟩
+    | .case (.inl _) ..  => .steps .case_inl
+    | .case (.inr _) ..  => .steps .case_inr
+    | .fst  (.pair ..)   => .steps .fst_pair
+    | .snd  (.pair ..)   => .steps .snd_pair
+    | .ap   (.lam _) _   => .steps .ap_lam
+    | .iter .zero ..     => .steps .iter_zero
+    | .iter (.succ _) .. => .steps .iter_succ
+
+    | .print _ => .steps .print
     | .read    => match I with
-                  | []     => .inr ⟨_, .read₁⟩
-                  | _ :: _ => .inr ⟨_, .read₂⟩
-
-instance : Subsingleton (Final S ⊕ Σ S', Steps S S') where
-  allEq S₁ S₂ := by
-    match S₁ with
-    | .inl V₁ =>
-      match S₂ with
-      | .inl V₂ =>
-        cases Subsingleton.elim V₁ V₂
-        rfl
-      | .inr ⟨S₂, s₂⟩ =>
-        nomatch V₁.not_steps s₂
-    | .inr ⟨S₁, s₁⟩ =>
-      match S₂ with
-      | .inl V₂ =>
-        nomatch V₂.not_steps s₁
-      | .inr ⟨S₂, s₂⟩ =>
-        cases Subsingleton.elim (α := Σ _, _) ⟨S₁, s₁⟩ ⟨S₂, s₂⟩
-        rfl
+                  | []     => .steps .read₁
+                  | _ :: _ => .steps .read₂
 
 inductive Reduces : (S S' : State A) → Type
   | refl                                       : Reduces S S
@@ -503,7 +615,7 @@ def trans : (r : Reduces S S') → (r' : Reduces S' S'') → Reduces S S''
 
 def lift {F : (S : State A) → State A'} (f : ∀ {S S'}, (s : Steps S S') → Steps (F S) (F S')) : (r : Reduces S S') → Reduces (F S) (F S')
   | refl     => refl
-  | step s r => step (f s) (r.lift f)
+  | step s r => step (f s) (r.lift @f)
 
 end Reduces
 
@@ -529,136 +641,207 @@ def translateExp : (M : CBV.Exp Γ A) → Modal.Exp Γ A
   | .succ   M       => .let (translateExp M) (.ret (.succ (.var .zero)))
   | .iter   M M₁ M₂ => .let (translateExp M) (.iter (.var .zero) (translateExp M₁).weaken (translateExp M₂).weaken₁)
 
-  | .print  M       => .let (translateExp M) (.print (.var .zero))
-  | .read           => .read
+  | .print M => .let (translateExp M) (.print (.var .zero))
+  | .read    => .read
 
 def translateState : (S : CBV.State A) → Modal.State A
   | (I, M, O) => (I, translateExp M, O)
 
-def translateSteps : (s : CBV.Steps S S') → Σ S'', Modal.Reduces (translateState S) S'' × Modal.Reduces (translateState S') S''
-  | .let    s => let ⟨_, r, r'⟩ := translateSteps s; ⟨_, .lift .let₁ r, .lift .let₁ r'⟩
-  | .absurd s => let ⟨_, r, r'⟩ := translateSteps s; ⟨_, .lift .let₁ r, .lift .let₁ r'⟩
-  | .inl    s => let ⟨_, r, r'⟩ := translateSteps s; ⟨_, .lift .let₁ r, .lift .let₁ r'⟩
-  | .inr    s => let ⟨_, r, r'⟩ := translateSteps s; ⟨_, .lift .let₁ r, .lift .let₁ r'⟩
-  | .case   s => let ⟨_, r, r'⟩ := translateSteps s; ⟨_, .lift .let₁ r, .lift .let₁ r'⟩
-  | .fst    s => let ⟨_, r, r'⟩ := translateSteps s; ⟨_, .lift .let₁ r, .lift .let₁ r'⟩
-  | .snd    s => let ⟨_, r, r'⟩ := translateSteps s; ⟨_, .lift .let₁ r, .lift .let₁ r'⟩
-  | .succ   s => let ⟨_, r, r'⟩ := translateSteps s; ⟨_, .lift .let₁ r, .lift .let₁ r'⟩
-  | .iter   s => let ⟨_, r, r'⟩ := translateSteps s; ⟨_, .lift .let₁ r, .lift .let₁ r'⟩
-  | .print  s => let ⟨_, r, r'⟩ := translateSteps s; ⟨_, .lift .let₁ r, .lift .let₁ r'⟩
+inductive TranslateSteps (S S' : CBV.State A)
+  | mk (r : Modal.Reduces (translateState S) S'') (r' : Modal.Reduces (translateState S') S'')
 
-  | .pair₁    s₁ => let ⟨_, r₁, r₁'⟩ := translateSteps s₁; ⟨_, .lift .let₁ r₁, .lift .let₁ r₁'⟩
-  | .pair₂ V₁ s₂ => let ⟨_, r₂, r₂'⟩ := translateSteps s₂; by dsimp [translateState, translateExp] at r₂ r₂' ⊢; sorry
-  | .ap₁      s  => let ⟨_, r, r'⟩ := translateSteps s; ⟨_, .lift .let₁ r, .lift .let₁ r'⟩
-  | .ap₂   V  s₁ => let ⟨_, r₁, r₁'⟩ := translateSteps s₁; by dsimp [translateState, translateExp] at r₁ r₁' ⊢; sorry
+def translateSteps : (s : CBV.Steps S S') → TranslateSteps S S'
+  | .let    s => let ⟨r, r'⟩ := translateSteps s; ⟨.lift .let₁ r, .lift .let₁ r'⟩
+  | .absurd s => let ⟨r, r'⟩ := translateSteps s; ⟨.lift .let₁ r, .lift .let₁ r'⟩
+  | .inl    s => let ⟨r, r'⟩ := translateSteps s; ⟨.lift .let₁ r, .lift .let₁ r'⟩
+  | .inr    s => let ⟨r, r'⟩ := translateSteps s; ⟨.lift .let₁ r, .lift .let₁ r'⟩
+  | .case   s => let ⟨r, r'⟩ := translateSteps s; ⟨.lift .let₁ r, .lift .let₁ r'⟩
+  | .fst    s => let ⟨r, r'⟩ := translateSteps s; ⟨.lift .let₁ r, .lift .let₁ r'⟩
+  | .snd    s => let ⟨r, r'⟩ := translateSteps s; ⟨.lift .let₁ r, .lift .let₁ r'⟩
+  | .succ   s => let ⟨r, r'⟩ := translateSteps s; ⟨.lift .let₁ r, .lift .let₁ r'⟩
+  | .iter   s => let ⟨r, r'⟩ := translateSteps s; ⟨.lift .let₁ r, .lift .let₁ r'⟩
+  | .print  s => let ⟨r, r'⟩ := translateSteps s; ⟨.lift .let₁ r, .lift .let₁ r'⟩
 
-  | .let'      V     => by dsimp [translateState, translateExp]; sorry
-  | .case_inl  V     => by dsimp [translateState, translateExp]; sorry
-  | .case_inr  V     => by dsimp [translateState, translateExp]; sorry
-  | .fst_pair  V₁ V₂ => by dsimp [translateState, translateExp]; sorry
-  | .snd_pair  V₁ V₂ => by dsimp [translateState, translateExp]; sorry
-  | .ap_lam    V₁    => by dsimp [translateState, translateExp]; sorry
-  | .iter_zero       => by dsimp [translateState, translateExp]; exact ⟨_, .step .let₂ (by simp [Modal.Exp.subst, Modal.Subst.applyE, Modal.Subst.applyV, Modal.Subst.cons]; refine .step .iter_zero ?_; sorry), .refl⟩
-  | .iter_succ V     => by dsimp [translateState, translateExp]; sorry
+  | .pair₁    s₁ => sorry
+  | .pair₂ V₁ s₂ => sorry
+  | .ap₁      s  => sorry
+  | .ap₂   V  s₁ => sorry
 
-  | .print' V => by dsimp [translateState, translateExp]; sorry
-  | .read₁    => ⟨_, .step .read₁ .refl, .step .let₂ .refl⟩
-  | .read₂    => by dsimp [translateState, translateExp]; sorry
+  | .let'      V     => sorry
+  | .case_inl  V     => sorry
+  | .case_inr  V     => sorry
+  | .fst_pair  V₁ V₂ => sorry
+  | .snd_pair  V₁ V₂ => sorry
+  | .ap_lam    V₁    => sorry
+  | .iter_zero       => sorry
+  | .iter_succ V     => sorry
+
+  | .print' V => sorry
+  | .read₁    => ⟨.step .read₁ .refl, .step .let₂ .refl⟩
+  | .read₂    => sorry
 
 end CBV_to_Modal
 
 namespace CBV_to_Modal'
 
-@[simp]
-def ret? : (M : Modal.Val Γ A ⊕ Modal.Exp Γ A) → Modal.Exp Γ A
-  | .inl V => .ret V
-  | .inr M => M
+inductive TranslateExp Γ A
+  | val (V : Modal.Val Γ A)
+  | exp (M : Modal.Exp Γ A)
 
 @[simp]
-def translateExp : (M : CBV.Exp Γ A) → Modal.Val Γ A ⊕ Modal.Exp Γ A
-  | .var x    => .inl (.var x)
-  | .let M M' => .inr (.let (ret? (translateExp M)) (ret? (translateExp M')))
+def TranslateExp.rename (γ : Modal.Renaming Γ Γ') : (M : TranslateExp Γ' A) → TranslateExp Γ A
+  | val V => val (V.rename γ)
+  | exp M => exp (M.rename γ)
 
-  | .absurd M       => .inr <|
-                       match translateExp M with
-                       | .inl V => .absurd V
-                       | .inr M => .let M (.absurd (.var .zero))
-  | .triv           => .inl .triv
-  | .inl    M       => match translateExp M with
-                       | .inl V => .inl (.inl V)
-                       | .inr M => .inr (.let M (.ret (.inl (.var .zero))))
-  | .inr    M       => match translateExp M with
-                       | .inl V => .inl (.inr V)
-                       | .inr M => .inr (.let M (.ret (.inr (.var .zero))))
-  | .case   M M₁ M₂ => .inr <|
-                       match translateExp M with
-                       | .inl V => .case V (ret? (translateExp M₁)) (ret? (translateExp M₂))
-                       | .inr M => .let M (.case (.var .zero) (ret? (translateExp M₁)).weaken₁ (ret? (translateExp M₂)).weaken₁)
-  | .pair   M₁ M₂   => match translateExp M₁, translateExp M₂ with
-                       | .inl V₁, .inl V₂ => .inl (.pair V₁ V₂)
-                       | .inr M₁, .inl V₂ => .inr (.let M₁ (.ret (.pair (.var .zero) V₂.weaken)))
-                       | .inl V₁, .inr M₂ => .inr (.let M₂ (.ret (.pair V₁.weaken (.var .zero))))
-                       | .inr M₁, .inr M₂ => .inr (.let M₁ (.let M₂.weaken (.ret (.pair (.var (.succ .zero)) (.var .zero)))))
-  | .fst    M       => .inr <|
-                       match translateExp M with
-                       | .inl V => .fst V
-                       | .inr M => .let M (.fst (.var .zero))
-  | .snd    M       => .inr <|
-                       match translateExp M with
-                       | .inl V => .snd V
-                       | .inr M => .let M (.snd (.var .zero))
-  | .lam    M       => .inl (.lam (ret? (translateExp M)))
-  | .ap     M M₁    => .inr <|
-                       match translateExp M, translateExp M₁ with
-                       | .inl V, .inl V₁ => .ap V V₁
-                       | .inr M, .inl V₁ => .let M (.ap (.var .zero) V₁.weaken)
-                       | .inl V, .inr M₁ => .let M₁ (.ap V.weaken (.var .zero))
-                       | .inr M, .inr M₁ => .let M (.let M₁.weaken (.ap (.var (.succ .zero)) (.var .zero)))
-  | .zero           => .inl .zero
-  | .succ   M       => match translateExp M with
-                       | .inl V => .inl (.succ V)
-                       | .inr M => .inr (.let M (.ret (.succ (.var .zero))))
-  | .iter   M M₁ M₂ => .inr <|
-                       match translateExp M with
-                       | .inl V => .iter V (ret? (translateExp M₁)) (ret? (translateExp M₂))
-                       | .inr M => .let M (.iter (.var .zero) (ret? (translateExp M₁)).weaken (ret? (translateExp M₂)).weaken₁)
+@[simp]
+def TranslateExp.subst (γ : Modal.Subst Γ Γ') : (M : TranslateExp Γ' A) → TranslateExp Γ A
+  | val V => val (V.subst γ)
+  | exp M => exp (M.subst γ)
 
-  | .print M => .inr <|
-                match translateExp M with
-                | .inl V => .print V
-                | .inr M => .let M (.print (.var .zero))
-  | .read    => .inr .read
+@[simp]
+def TranslateExp.toExp : (M : TranslateExp Γ A) → Modal.Exp Γ A
+  | val V => .ret V
+  | exp M => M
 
-def translateVal : (V : CBV.Val M) → { V // translateExp M = .inl V }
-  | .triv       => ⟨_, rfl⟩
-  | .inl  V     => ⟨_, by rw [translateExp, (translateVal V).property]⟩
-  | .inr  V     => ⟨_, by rw [translateExp, (translateVal V).property]⟩
-  | .pair V₁ V₂ => ⟨_, by rw [translateExp, (translateVal V₁).property, (translateVal V₂).property]⟩
-  | .lam        => ⟨_, rfl⟩
-  | .zero       => ⟨_, rfl⟩
-  | .succ V     => ⟨_, by rw [translateExp, (translateVal V).property]⟩
+@[simp]
+def TranslateExp.then
+  (val : (V : Modal.Val Γ A) → TranslateExp Γ' A')
+  (exp : (M : Modal.Exp Γ A) → Modal.Exp Γ' A')
+: (M : TranslateExp Γ A) → TranslateExp Γ' A'
+  | .val V => val V
+  | .exp M => .exp (exp M)
 
-def ofTranslateVal (eq : translateExp M = .inl V) : CBV.Val M :=
+@[simp]
+def TranslateExp.then'
+  (val : (V : Modal.Val Γ A) → Modal.Exp Γ' A')
+  (exp : (M : Modal.Exp Γ A) → Modal.Exp Γ' A')
+: (M : TranslateExp Γ A) → Modal.Exp Γ' A'
+  | .val V => val V
+  | .exp M => exp M
+
+@[simp]
+def translateExp : (M : CBV.Exp Γ A) → TranslateExp Γ A
+  | .var x    => .val <| .var x
+  | .let M M' => .exp <| .let (translateExp M).toExp (translateExp M').toExp
+
+  | .absurd M       => .exp <| translateExp M |>.then' .absurd (.let · (.absurd (.var .zero)))
+  | .triv           => .val .triv
+  | .inl    M       => translateExp M |>.then (.val <| .inl ·) (.let · (.ret (.inl (.var .zero))))
+  | .inr    M       => translateExp M |>.then (.val <| .inr ·) (.let · (.ret (.inr (.var .zero))))
+  | .case   M M₁ M₂ => .exp <| translateExp M |>.then'
+                         (.case · (translateExp M₁).toExp (translateExp M₂).toExp)
+                         (.let · (.case (.var .zero) (translateExp M₁).toExp.weaken₁ (translateExp M₂).toExp.weaken₁))
+  | .pair   M₁ M₂   => translateExp M₁ |>.then
+                         (fun V₁ => translateExp M₂ |>.then (.val <| .pair V₁ ·) (.let · (.ret (.pair V₁.weaken (.var .zero)))))
+                         (.let · <| translateExp M₂ |>.then'
+                           (.ret <| .pair (.var .zero) ·.weaken)
+                           (.let ·.weaken (.ret (.pair (.var (.succ .zero)) (.var .zero)))))
+  | .fst    M       => .exp <| translateExp M |>.then' .fst (.let · (.fst (.var .zero)))
+  | .snd    M       => .exp <| translateExp M |>.then' .snd (.let · (.snd (.var .zero)))
+  | .lam    M       => .val <| .lam (translateExp M).toExp
+  | .ap     M M₁    => .exp <| translateExp M |>.then'
+                         (fun V => translateExp M₁ |>.then' (.ap V ·) (.let · (.ap V.weaken (.var .zero))))
+                         (.let · <| translateExp M₁ |>.then'
+                           (.ap (.var .zero) ·.weaken)
+                           (.let ·.weaken (.ap (.var (.succ .zero)) (.var .zero))))
+  | .zero           => .val .zero
+  | .succ   M       => translateExp M |>.then (.val <| .succ ·) (.let · (.ret (.succ (.var .zero))))
+  | .iter   M M₁ M₂ => .exp <| translateExp M |>.then'
+                         (.iter · (translateExp M₁).toExp (translateExp M₂).toExp)
+                         (.let · (.iter (.var .zero) (translateExp M₁).toExp.weaken (translateExp M₂).toExp.weaken₁))
+
+  | .print M => .exp <| translateExp M |>.then' .print (.let · (.print (.var .zero)))
+  | .read    => .exp .read
+
+@[simp]
+def translateVal : (V : @CBV.Val Γ A M) → Modal.Val Γ A
+  | .var  x     => .var x
+  | .triv       => .triv
+  | .inl  V     => .inl  (translateVal V)
+  | .inr  V     => .inr  (translateVal V)
+  | .pair V₁ V₂ => .pair (translateVal V₁) (translateVal V₂)
+  | .lam  M     => .lam  (translateExp M).toExp
+  | .zero       => .zero
+  | .succ V     => .succ (translateVal V)
+
+theorem translateExpVal (V : CBV.Val M) : translateExp M = .val (translateVal V) :=
+  by induction V <;> simp [*]
+
+def ofTranslateVal (isVal : translateExp M = .val V) : CBV.Val M :=
   match M with
+  | .var  x     => .var x
   | .triv       => .triv
   | .inl  M     => match h : translateExp M with
-                   | .inl V => .inl (ofTranslateVal h)
-                   | .inr M => by rw [translateExp, h] at eq; nomatch eq
+                   | .val V => .inl (ofTranslateVal h)
+                   | .exp M => by rw [translateExp, h] at isVal; nomatch isVal
   | .inr  M     => match h : translateExp M with
-                   | .inl V => .inr (ofTranslateVal h)
-                   | .inr M => by rw [translateExp, h] at eq; nomatch eq
+                   | .val V => .inr (ofTranslateVal h)
+                   | .exp M => by rw [translateExp, h] at isVal; nomatch isVal
   | .pair M₁ M₂ => match h₁ : translateExp M₁, h₂ : translateExp M₂ with
-                   | .inl V₁, .inl V₂ => .pair (ofTranslateVal h₁) (ofTranslateVal h₂)
-                   | .inr M₁, .inl V₂ | .inl V₁, .inr M₂ | .inr M₁, .inr M₂ => by rw [translateExp, h₁, h₂] at eq; nomatch eq
-  | .lam  M     => .lam
+                   | .val V₁, .val V₂ => .pair (ofTranslateVal h₁) (ofTranslateVal h₂)
+                   | .val V₁, .exp M₂ | .exp M₁, _ => by rw [translateExp, h₁, h₂] at isVal; nomatch isVal
+  | .lam  M     => .lam M
   | .zero       => .zero
   | .succ M     => match h : translateExp M with
-                   | .inl V => .succ (ofTranslateVal h)
-                   | .inr M => by rw [translateExp, h] at eq; nomatch eq
+                   | .val V => .succ (ofTranslateVal h)
+                   | .exp M => by rw [translateExp, h] at isVal; nomatch isVal
 
 @[simp]
 def translateState : (S : CBV.State A) → Modal.State A
-  | (I, M, O) => (I, ret? (translateExp M), O)
+  | (I, M, O) => (I, (translateExp M).toExp, O)
+
+@[simp]
+def translateSubst : (γ : CBV.Subst Γ Γ') → Modal.Subst Γ Γ'
+  | .nil      => .nil
+  | .cons γ M => .cons (translateSubst γ) (translateVal M)
+
+@[simp]
+theorem translateExp_rename {γ : CBV.Renaming Γ Γ'} : translateExp (M.rename γ) = (translateExp M).rename γ := by
+  induction M generalizing Γ
+    <;> simp [*]
+  repeat all_goals split <;> split at ‹_› <;> cases ‹_› <;> simp
+  all_goals simp [CBV.Renaming.map_rename.symm]
+
+@[simp]
+theorem translateVal_rename : translateVal (V.rename γ) = (translateVal V).rename γ := by
+  induction V
+    <;> simp [*]
+  case lam M => cases translateExp M <;> rfl
+
+@[simp]
+theorem translateSubst_map_weaken : translateSubst (γ.map .weaken) = (translateSubst γ).map (.weaken (A' := A)) := by
+  induction γ with
+  | nil => rfl
+  | cons ih => simp [*]; simp [CBV.Val.weaken]
+
+@[simp]
+theorem translateExp_substVar : translateExp (CBV.Var.subst γ x) = .val (Modal.Var.subst (translateSubst γ) x) :=
+  by induction x <;> cases γ <;> simp [*, translateExpVal ‹_›]
+
+@[simp]
+theorem translateExp_subst {γ : CBV.Subst Γ Γ'} : translateExp (M.subst γ) = (translateExp M).subst (translateSubst γ) := by
+  induction M generalizing Γ
+    <;> simp [*]
+    <;> repeat split <;> split at ‹_› <;> cases ‹_› <;> simp
+
+@[simp]
+theorem translateSubst_id (f : ∀ {A}, CBV.Var A Γ → CBV.Var A Γ') : translateSubst (.ofRenaming (.var <| f ·) .id) = .ofRenaming (.var <| f ·) .id :=
+  by induction Γ <;> simp [*]
+
+@[simp]
+theorem translateExp_sub : (translateExp (M.sub V)).toExp = (translateExp M).toExp.sub (translateVal V) := by
+  simp [CBV.Exp.sub, translateSubst_id (·)]
+  cases translateExp M <;> rfl
+
+@[simp]
+theorem translateExp_ofNat : translateExp (.ofNat n) = .val (.ofNat (Γ := Γ) n) :=
+  by induction n <;> simp! [*]
+
+@[simp]
+theorem translateVal_toNat : (translateVal V).toNat = V.toNat :=
+  match V with
+  | .zero   => rfl
+  | .succ _ => by simp; exact translateVal_toNat
 
 def translateSteps : (s : CBV.Steps S S') → Modal.Reduces (translateState S) (translateState S')
   | .let    s => .lift .let₁ <| translateSteps s
@@ -666,129 +849,139 @@ def translateSteps : (s : CBV.Steps S S') → Modal.Reduces (translateState S) (
                    have := translateSteps s
                    dsimp at this ⊢
                    split at this
-                   next h => nomatch flip CBV.Final.not_steps s (ofTranslateVal h)
-                   next h =>
-                     rw [h]
-                     split at this <;> rename_i h <;> rw [h]
+                   . nomatch flip CBV.Final.not_steps s (ofTranslateVal ‹_›)
+                   . split at this
                      . exact .trans (.lift .let₁ this) (.step .let₂ .refl)
                      . exact .lift .let₁ this
   | .inl    s => by
                    have := translateSteps s
                    dsimp at this ⊢
                    split at this
-                   next h => nomatch flip CBV.Final.not_steps s (ofTranslateVal h)
-                   next =>
-                     split at this
+                   . nomatch flip CBV.Final.not_steps s (ofTranslateVal ‹_›)
+                   . split at this
                      . exact .trans (.lift .let₁ this) (.step .let₂ .refl)
                      . exact .lift .let₁ this
   | .inr    s => by
                    have := translateSteps s
                    dsimp at this ⊢
                    split at this
-                   next h => nomatch flip CBV.Final.not_steps s (ofTranslateVal h)
-                   next =>
-                     split at this
+                   . nomatch flip CBV.Final.not_steps s (ofTranslateVal ‹_›)
+                   . split at this
                      . exact .trans (.lift .let₁ this) (.step .let₂ .refl)
                      . exact .lift .let₁ this
   | .case   s => by
                    have := translateSteps s
                    dsimp at this ⊢
                    split at this
-                   next h => nomatch flip CBV.Final.not_steps s (ofTranslateVal h)
-                   next h =>
-                     rw [h]
-                     split at this <;> rename_i h <;> rw [h]
-                     . exact .trans (.lift .let₁ this) (.step .let₂ <| by dsimp; simp; exact .refl)
+                   . nomatch flip CBV.Final.not_steps s (ofTranslateVal ‹_›)
+                   . split at this
+                     . exact .trans (.lift .let₁ this) (.step .let₂ <| by simp; exact .refl)
                      . exact .lift .let₁ this
   | .fst    s => by
                    have := translateSteps s
                    dsimp at this ⊢
                    split at this
-                   next h => nomatch flip CBV.Final.not_steps s (ofTranslateVal h)
-                   next h =>
-                     rw [h]
-                     split at this <;> rename_i h <;> rw [h]
+                   . nomatch flip CBV.Final.not_steps s (ofTranslateVal ‹_›)
+                   . split at this
                      . exact .trans (.lift .let₁ this) (.step .let₂ .refl)
                      . exact .lift .let₁ this
   | .snd    s => by
                    have := translateSteps s
                    dsimp at this ⊢
                    split at this
-                   next h => nomatch flip CBV.Final.not_steps s (ofTranslateVal h)
-                   next h =>
-                     rw [h]
-                     split at this <;> rename_i h <;> rw [h]
+                   . nomatch flip CBV.Final.not_steps s (ofTranslateVal ‹_›)
+                   . split at this
                      . exact .trans (.lift .let₁ this) (.step .let₂ .refl)
                      . exact .lift .let₁ this
   | .succ   s => by
                    have := translateSteps s
                    dsimp at this ⊢
                    split at this
-                   next h => nomatch flip CBV.Final.not_steps s (ofTranslateVal h)
-                   next h =>
-                     rw [h]
-                     split at this <;> rename_i h <;> rw [h]
+                   . nomatch flip CBV.Final.not_steps s (ofTranslateVal ‹_›)
+                   . split at this
                      . exact .trans (.lift .let₁ this) (.step .let₂ .refl)
                      . exact .lift .let₁ this
   | .iter   s => by
                    have := translateSteps s
                    dsimp at this ⊢
                    split at this
-                   next h => nomatch flip CBV.Final.not_steps s (ofTranslateVal h)
-                   next h =>
-                     rw [h]
-                     split at this <;> rename_i h <;> rw [h]
-                     . exact .trans (.lift .let₁ this) (.step .let₂ <| by dsimp; simp; exact .refl)
+                   . nomatch flip CBV.Final.not_steps s (ofTranslateVal ‹_›)
+                   . split at this
+                     . exact .trans (.lift .let₁ this) (.step .let₂ <| by simp; exact .refl)
                      . exact .lift .let₁ this
   | .print  s => by
                    have := translateSteps s
                    dsimp at this ⊢
                    split at this
-                   next h => nomatch flip CBV.Final.not_steps s (ofTranslateVal h)
-                   next h =>
-                     rw [h]
-                     split at this <;> rename_i h <;> rw [h]
+                   . nomatch flip CBV.Final.not_steps s (ofTranslateVal ‹_›)
+                   . split at this
                      . exact .trans (.lift .let₁ this) (.step .let₂ .refl)
                      . exact .lift .let₁ this
 
   | .pair₁    s₁ => by
                       have := translateSteps s₁
                       dsimp at this ⊢
-                      split <;> rename_i h <;> split at h <;> cases h
-                      next h _ => nomatch flip CBV.Final.not_steps s₁ (ofTranslateVal h)
-                      next h h' =>
-                        rw [h] at this
-                        rw [h']
-                        split <;> rename_i h <;> split at h <;> cases h <;> rename_i h <;> cases h <;> rename_i h <;> rw [h] at this
-                        . dsimp at this ⊢
-                          exact .trans (.lift .let₁ this) (.step .let₂ <| by dsimp; simp; exact .refl)
+                      split at this
+                      . nomatch flip CBV.Final.not_steps s₁ (ofTranslateVal ‹_›)
+                      . split at this
+                        . split
+                          . exact .trans (.lift .let₁ this) (.step .let₂ <| by simp; exact .refl)
+                          . exact .trans (.lift .let₁ this) (.step .let₂ <| by simp; exact .refl)
                         . exact .lift .let₁ this
-                      next h _ => nomatch flip CBV.Final.not_steps s₁ (ofTranslateVal h)
-                      next h h' =>
-                        rw [h] at this
-                        rw [h']
-                        split <;> rename_i h <;> split at h <;> cases h <;> rename_i h <;> cases h <;> rename_i h <;> rw [h] at this
-                        . dsimp at this ⊢
-                          exact .trans (.lift .let₁ this) (.step .let₂ <| by dsimp; simp; exact .refl)
+  | .pair₂ V₁ s₂ => by
+                      have := translateSteps s₂
+                      simp [translateExpVal V₁] at this ⊢
+                      split at this
+                      . nomatch flip CBV.Final.not_steps s₂ (ofTranslateVal ‹_›)
+                      . split at this
+                        . exact .trans (.lift .let₁ this) (.step .let₂ <| by simp; exact .refl)
                         . exact .lift .let₁ this
-  | .pair₂ V₁ s₂ => by dsimp; sorry
   | .ap₁      s  => by
                       have := translateSteps s
                       dsimp at this ⊢
-                      sorry
-  | .ap₂   V  s₁ => by dsimp; sorry
+                      split at this
+                      . nomatch flip CBV.Final.not_steps s (ofTranslateVal ‹_›)
+                      . split at this
+                        . split
+                          . exact .trans (.lift .let₁ this) (.step .let₂ <| by simp; exact .refl)
+                          . exact .trans (.lift .let₁ this) (.step .let₂ <| by simp; exact .refl)
+                        . exact .lift .let₁ this
+  | .ap₂   V  s₁ => by
+                      have := translateSteps s₁
+                      simp [translateExpVal V] at this ⊢
+                      split at this
+                      . nomatch flip CBV.Final.not_steps s₁ (ofTranslateVal ‹_›)
+                      . split at this
+                        . exact .trans (.lift .let₁ this) (.step .let₂ <| by simp; exact .refl)
+                        . exact .lift .let₁ this
 
-  | .let'      V     => by dsimp; sorry
-  | .case_inl  V     => by dsimp; sorry
-  | .case_inr  V     => by dsimp; sorry
-  | .fst_pair  V₁ V₂ => by dsimp; sorry
-  | .snd_pair  V₁ V₂ => by dsimp; sorry
-  | .ap_lam    V₁    => by dsimp; sorry
-  | .iter_zero       => by dsimp; sorry
-  | .iter_succ V     => by dsimp; sorry
+  | .let'      V     => by
+                          simp [translateExpVal V, -TranslateExp.toExp]
+                          exact .step .let₂ .refl
+  | .case_inl  V     => by
+                          simp [translateExpVal V, -TranslateExp.toExp]
+                          exact .step .case_inl .refl
+  | .case_inr  V     => by
+                          simp [translateExpVal V, -TranslateExp.toExp]
+                          exact .step .case_inr .refl
+  | .fst_pair  V₁ V₂ => by
+                          simp [translateExpVal V₁, translateExpVal V₂]
+                          exact .step .fst_pair .refl
+  | .snd_pair  V₁ V₂ => by
+                          simp [translateExpVal V₁, translateExpVal V₂]
+                          exact .step .snd_pair .refl
+  | .ap_lam    V₁    => by
+                          simp [translateExpVal V₁, -TranslateExp.toExp]
+                          exact .step .ap_lam .refl
+  | .iter_zero       => .step .iter_zero .refl
+  | .iter_succ V     => by
+                          simp [translateExpVal V]
+                          exact .step .iter_succ .refl
 
-  | .print' V => by dsimp; sorry
+  | .print' V => by
+                   simp [translateExpVal V]
+                   exact .step .print <| by simp; exact .refl
   | .read₁    => .step .read₁ .refl
-  | .read₂    => by dsimp; sorry
+  | .read₂    => .step .read₂ <| by simp; exact .refl
 
 end CBV_to_Modal'
